src/prop/ReorderPromiseSame.v
@@ -309,7 +309,7 @@ Lemma promise_step_nonsynch_loc_inv
       lc1 mem1 loc from to msg lc2 mem2 kind l
       (WF1: Local.wf lc1 mem1)
       (STEP: Local.promise_step lc1 mem1 loc from to msg lc2 mem2 kind)
-      (NONPF: Memory.op_kind_is_lower kind = false \/ ~ Message.is_released_none msg)
+      (NONPF: Memory.op_kind_is_lower_full kind = false \/ ~ Message.is_released_none msg)
       (NONSYNCH: Memory.nonsynch_loc l lc2.(Local.promises)):
   Memory.nonsynch_loc l lc1.(Local.promises).
 Proof.
@@ -325,10 +325,13 @@ Proof.
     + i. des. subst. exploit NONSYNCH; eauto.
       destruct msg; destruct msg0; ss.
       * i. subst. unguard. des; ss.
+        exploit Memory.lower_get0; try exact MEM. i. des.
+        inv WF1. exploit PROMISES0; eauto. i.
+        rewrite GET0 in x. inv x. ss.
       * exploit Memory.lower_get0; try exact PROMISES. i. des.
         rewrite GET in GET0. inv GET0.
         inv MEM. inv LOWER. inv MSG_LE0.
-    + guardH o. rewrite GET. i. exploit NONSYNCH; eauto.
+    + rewrite GET. i. exploit NONSYNCH; eauto.
 Qed.
 
 Lemma reorder_promise_write
@@ -339,7 +342,7 @@ Lemma reorder_promise_write
       loc2 from2 to2 val2 releasedm2 released2 ord2 kind2
       (STEP1: Local.promise_step lc0 mem0 loc1 from1 to1 msg1 lc1 mem1 kind1)
       (STEP2: Local.write_step lc1 sc0 mem1 loc2 from2 to2 val2 releasedm2 released2 ord2 lc2 sc2 mem2 kind2)
-      (NONPF: Memory.op_kind_is_lower kind1 = false \/ ~ Message.is_released_none msg1)
+      (NONPF: Memory.op_kind_is_lower_full kind1 = false \/ ~ Message.is_released_none msg1)
       (REL_WF: View.opt_wf releasedm2)
       (REL_CLOSED: Memory.closed_opt_view releasedm2 mem0)
       (LOCAL0: Local.wf lc0 mem0)
@@ -396,7 +399,7 @@ Lemma reorder_promise_write'
       loc2 from2 to2 val2 releasedm2 released2 ord2 kind2
       (STEP1: Local.promise_step lc0 mem0 loc1 from1 to1 msg1 lc1 mem1 kind1)
       (STEP2: Local.write_step lc1 sc0 mem1 loc2 from2 to2 val2 releasedm2 released2 ord2 lc2 sc2 mem2 kind2)
-      (NONPF: Memory.op_kind_is_lower kind1 = false \/ ~ Message.is_released_none msg1)
+      (NONPF: Memory.op_kind_is_lower_full kind1 = false \/ ~ Message.is_released_none msg1)
       (REL_WF: View.opt_wf releasedm2)
       (REL_CLOSED: Memory.closed_opt_view releasedm2 mem0)
       (LOCAL0: Local.wf lc0 mem0)
@@ -526,7 +529,7 @@ Lemma reorder_nonpf_pf
 Proof.
   inv STEP2; ss.
   - inv STEP. ss. symmetry in PF. apply promise_pf_inv in PF. des. subst.
-    destruct msg; ss. destruct released; ss.
+    destruct msg; ss. destruct released0; ss.
     inv STEP1. inv STEP. ss.
     exploit reorder_promise_promise_lower_None; eauto. i. des; subst.
     + left. esplits.
